feat: implement ult and ule

LeanSAT/Reflect/BVExpr/BitBlast/Impl/Pred.lean
@@ -1,4 +1,6 @@
 import LeanSAT.Reflect.BVExpr.BitBlast.Impl.Eq
+import LeanSAT.Reflect.BVExpr.BitBlast.Impl.Ult
+import LeanSAT.Reflect.BVExpr.BitBlast.Impl.Ule
 import LeanSAT.Reflect.BVExpr.BitBlast.Impl.GetLsb
 
 namespace BVPred
@@ -8,14 +10,16 @@ def bitblast (aig : AIG BVBit) (pred : BVPred) : AIG.Entrypoint BVBit :=
   | .bin lhs op rhs =>
     match op with
     | .eq => mkEq aig ⟨lhs, rhs⟩
+    | .ult => mkUlt aig ⟨lhs, rhs⟩
+    | .ule => mkUle aig ⟨lhs, rhs⟩
   | .getLsb expr idx => blastGetLsb aig ⟨expr, idx⟩
 
 theorem bitblast_le_size (aig : AIG BVBit) (pred : BVPred)
     : aig.decls.size ≤ (bitblast aig pred).aig.decls.size := by
   cases pred with
   | bin lhs op rhs =>
-    cases op with
-    | eq =>
+    cases op
+    all_goals
       simp only [bitblast]
       apply AIG.LawfulOperator.le_size
   | getLsb expr idx =>
@@ -31,6 +35,12 @@ theorem bitblast_decl_eq (aig : AIG BVBit) (pred : BVPred) {h : idx < aig.decls.
     | eq =>
       simp only [bitblast]
       rw [AIG.LawfulOperator.decl_eq (f := mkEq)]
+    | ult =>
+      simp only [bitblast]
+      rw [AIG.LawfulOperator.decl_eq (f := mkUlt)]
+    | ule =>
+      simp only [bitblast]
+      rw [AIG.LawfulOperator.decl_eq (f := mkUle)]
   | getLsb expr idx =>
     simp only [bitblast]
     rw [AIG.LawfulOperator.decl_eq (f := blastGetLsb)]
