LeanSAT/Reflect/BVExpr/BitBlast/Lemmas/Pred.lean
@@ -1,4 +1,6 @@
 import LeanSAT.Reflect.BVExpr.BitBlast.Lemmas.Eq
+import LeanSAT.Reflect.BVExpr.BitBlast.Lemmas.Ult
+import LeanSAT.Reflect.BVExpr.BitBlast.Lemmas.Ule
 import LeanSAT.Reflect.BVExpr.BitBlast.Lemmas.GetLsb
 import LeanSAT.Reflect.BVExpr.BitBlast.Impl.Pred
 
@@ -15,6 +17,8 @@ theorem bitblast_denote_eq_eval (aig : AIG BVBit) (pred : BVPred) (assign : BVEx
   | bin lhs op rhs =>
     cases op with
     | eq => simp [bitblast]
+    | ult => simp [bitblast]
+    | ule => simp [bitblast]
   | getLsb expr idx =>
     simp [bitblast]
 
